spec/sail/lean/Out/Defs.lean
@@ -56,7 +56,7 @@ inductive PSTATEWriteTarget where | PSTATEWriteTarget_DAIFSet
   deriving BEq, Inhabited, Repr
   open PSTATEWriteTarget
 
-inductive SystemRegisterWriteTarget where | SystemRegisterWriteTarget_VTTBR_EL2 | SystemRegisterWriteTarget_VTCR_EL2 | SystemRegisterWriteTarget_CNTHCTL_EL2 | SystemRegisterWriteTarget_CNTVOFF_EL2 | SystemRegisterWriteTarget_SP_EL1 | SystemRegisterWriteTarget_ELR_EL2 | SystemRegisterWriteTarget_HCR_EL2
+inductive SystemRegisterWriteTarget where | SystemRegisterWriteTarget_VTTBR_EL2 | SystemRegisterWriteTarget_VTCR_EL2 | SystemRegisterWriteTarget_CNTHCTL_EL2 | SystemRegisterWriteTarget_CNTVOFF_EL2 | SystemRegisterWriteTarget_SP_EL1 | SystemRegisterWriteTarget_ELR_EL2 | SystemRegisterWriteTarget_SPSR_EL2 | SystemRegisterWriteTarget_HCR_EL2
   deriving BEq, Inhabited, Repr
   open SystemRegisterWriteTarget
 
